Make translator know that VfromList does not use refs

translator/ml_translatorScript.sml
@@ -2544,6 +2544,7 @@ Definition no_change_refs_def:
   no_change_refs (Lannot e _) = no_change_refs e /\
   no_change_refs (Mat e pats) =
     (no_change_refs e /\ EVERY no_change_refs (MAP SND pats)) /\
+  no_change_refs (App p es) = (p = VfromList ∧ EVERY no_change_refs es) /\
   no_change_refs _ = F
 Termination
   WF_REL_TAC `measure exp_size`
@@ -2554,116 +2555,26 @@ Termination
   \\ rw [] \\ res_tac \\ fs []
 End
 
+Theorem evaluate_no_change_refs:
+  (∀(s:'ffi state) env es s1 vs.
+     evaluate s env es = (s1,Rval vs) ∧ EVERY no_change_refs es ⇒
+     s1.refs = s.refs) ∧
+  (∀(s:'ffi state) env v pes errv s1 vs.
+     evaluate_match s env v pes errv = (s1,Rval vs) ∧ EVERY no_change_refs (MAP SND pes) ⇒
+     s1.refs = s.refs)
+Proof
+  ho_match_mp_tac evaluate_ind
+  \\ fs [no_change_refs_def] \\ rw []
+  \\ gvs [evaluate_def,AllCaseEqs(),semanticPrimitivesTheory.do_if_def]
+  \\ fs [SF ETA_ss]
+  \\ gvs [do_app_def,AllCaseEqs()]
+QED
+
 Theorem eval_rel_no_change_refs:
   !exp s1 s2 env res.
     eval_rel s1 env exp s2 res /\ no_change_refs exp ==> s1.refs = s2.refs
 Proof
-  recInduct no_change_refs_ind
-  \\ rw [] \\ fs [no_change_refs_def]
-  \\ fs [eval_rel_def,evaluate_def,CaseEq"option",pair_case_eq,CaseEq"result",CaseEq"bool"]
-  \\ rveq \\ fs []
-  \\ fs [state_component_equality,PULL_EXISTS]
-  \\ res_tac \\ fs []
-  THEN1
-   (imp_res_tac evaluate_sing \\ rveq \\ fs [] \\ rveq \\ fs []
-    \\ last_x_assum (qspecl_then
-         [`s1`,`st' with clock := s1.clock`,`env`,`v''`,`ck1`,`st'.clock`] mp_tac)
-    \\ fs [with_same_clock]
-    \\ first_x_assum (qspecl_then
-         [`st'`,`s2 with clock := st'.clock`,`env with v := nsOptBind v4 v'' env.v`,
-            `res`,`st'.clock`,`ck2`] mp_tac)
-    \\ fs [with_same_clock])
-  \\ fs [do_if_def,CaseEq"bool"] \\ rveq \\ fs []
-  \\ imp_res_tac evaluate_sing \\ rveq \\ fs [] \\ rveq \\ fs []
-  THEN1
-   (last_x_assum (qspecl_then
-         [`s1`,`st' with clock := s1.clock`,`env`,`Boolv T`,`ck1`,`st'.clock`] mp_tac)
-    \\ fs [with_same_clock]
-    \\ last_x_assum (qspecl_then
-         [`st'`,`s2 with clock := st'.clock`,`env`,`res`,`st'.clock`,`ck2`] mp_tac)
-    \\ fs [with_same_clock])
-  THEN1
-   (last_x_assum (qspecl_then
-         [`s1`,`st' with clock := s1.clock`,`env`,`Boolv F`,`ck1`,`st'.clock`] mp_tac)
-    \\ fs [with_same_clock]
-    \\ last_x_assum (qspecl_then
-         [`st'`,`s2 with clock := st'.clock`,`env`,`res`,`st'.clock`,`ck2`] mp_tac)
-    \\ last_x_assum (qspecl_then
-         [`st'`,`s2 with clock := st'.clock`,`env`,`res`,`st'.clock`,`ck2`] mp_tac)
-    \\ fs [with_same_clock])
-  THEN1
-   (fs [EVERY_MEM]
-    \\ `!a. MEM a es <=> MEM a (REVERSE es)` by fs []
-    \\ rename [`evaluate _ _ ys = _`] \\ fs []
-    \\ pop_assum kall_tac
-    \\ pop_assum mp_tac
-    \\ pop_assum kall_tac
-    \\ pop_assum mp_tac
-    \\ pop_assum kall_tac
-    \\ pop_assum mp_tac
-    \\ pop_assum mp_tac
-    \\ qid_spec_tac `s1`
-    \\ qid_spec_tac `s2`
-    \\ qid_spec_tac `ck1`
-    \\ qid_spec_tac `ck2`
-    \\ qid_spec_tac `vs`
-    \\ qid_spec_tac `ys`
-    \\ Induct
-    THEN1 (fs [evaluate_def,state_component_equality])
-    \\ rewrite_tac [GSYM AND_IMP_INTRO] \\ rpt gen_tac \\ strip_tac
-    \\ once_rewrite_tac [evaluate_cons]
-    \\ fs [CaseEq"result",pair_case_eq] \\ rpt strip_tac
-    \\ rveq \\ fs []
-    \\ fs [PULL_FORALL]
-    \\ imp_res_tac evaluate_sing \\ rveq \\ fs [] \\ rveq \\ fs []
-    \\ first_assum (qspecl_then [`h`,`s1`,`s' with clock := s1.clock`,
-          `env`,`v`,`ck1`,`s'.clock`] mp_tac)
-    \\ simp_tac (srw_ss()) [] \\ asm_rewrite_tac []
-    \\ simp_tac (srw_ss()) [] \\ asm_rewrite_tac [with_same_clock]
-    \\ strip_tac
-    \\ `s1.refs = (s' with clock := s2.clock).refs` by
-               (simp_tac (srw_ss()) [] \\ asm_rewrite_tac [])
-    \\ pop_assum (fn th => rewrite_tac [th])
-    \\ last_x_assum (match_mp_tac o MP_CANON) \\ fs []
-    \\ qexists_tac `vs''`
-    \\ qexists_tac `ck2`
-    \\ qexists_tac `s'.clock`
-    \\ asm_rewrite_tac [with_same_clock]
-    \\ metis_tac [])
-  THEN1
-   (fs [EVERY_MEM]
-    \\ pop_assum kall_tac
-    \\ first_x_assum (qspecl_then [`s1`,`st' with clock := s1.clock`,
-          `env`,`v'`,`ck1`,`st'.clock`] mp_tac)
-    \\ simp [with_same_clock] \\ strip_tac
-    \\ pop_assum kall_tac
-    \\ pop_assum mp_tac
-    \\ pop_assum kall_tac
-    \\ pop_assum mp_tac
-    \\ pop_assum kall_tac
-    \\ pop_assum kall_tac
-    \\ pop_assum kall_tac
-    \\ pop_assum mp_tac
-    \\ qid_spec_tac `st'`
-    \\ qid_spec_tac `s2`
-    \\ qid_spec_tac `ck2`
-    \\ qid_spec_tac `res`
-    \\ qid_spec_tac `pats`
-    \\ Induct
-    THEN1 (fs [evaluate_def,state_component_equality])
-    \\ Cases
-    \\ rewrite_tac [GSYM AND_IMP_INTRO] \\ rpt gen_tac \\ strip_tac
-    \\ once_rewrite_tac [evaluate_def]
-    \\ fs [CaseEq"result",pair_case_eq,CaseEq"bool",CaseEq"match_result"] \\ rpt strip_tac
-    THEN1
-     (last_x_assum (match_mp_tac o MP_CANON) \\ fs []
-      \\ fs [state_component_equality]
-      \\ metis_tac [])
-    \\ qsuff_tac `(st' with clock := s2.clock).refs = s2.refs`
-    THEN1 (simp_tac (srw_ss()) [])
-    \\ first_x_assum (match_mp_tac o MP_CANON)
-    \\ last_x_assum kall_tac \\ qexists_tac `r` \\ simp []
-    \\ metis_tac [with_same_clock])
+  rw [eval_rel_def] \\ imp_res_tac evaluate_no_change_refs \\ fs []
 QED
 
 Theorem Eval_constant:
